vips proofs

LeanVips/Basic.lean
@@ -307,18 +307,6 @@ theorem tofrom (i: Instr) : fromBv32 (toBv32 i) = i := by
     rw [jt2]
     rfl
 
-
-
-
-
-
-
-
-
-
-
-
-
 -- Instruction memory
 abbrev IMem : Type := Array Instr
 deriving instance Repr for IMem
@@ -368,8 +356,6 @@ def eval (im: IMem) (fuel: Nat) (pc: Bv32) (rf:Regfile) (dm: DMem): Regfile × D
     let (rf, dm, pc) := instr_eval (instr im pc) pc rf dm
     eval im fu (pc + 4) rf dm
 
-def pc : Bv32 := 4
-def rf: Regfile := Vector.mkVector 32 0
 def imem : IMem := #[
   bne  t1 zero 4,    --00 -- if t1 != 0 brach to 14
   addi t0 t0 0x20,   --04
@@ -380,6 +366,106 @@ def imem : IMem := #[
   andi t4 t3 0xFFFF, --18
   ori  t5 t3 0xFFFF  --20
 ]
+
+-- we define an initial state for our VM
+def rf:  Regfile := Vector.mkVector 32 0
 def dm : DMem := #[]
 
-#eval (eval imem 9 0 rf dm)
+#eval (eval imem 9 0 rf dm) -- state after executing 9 instructions
+
+-- lets try some simple proofs by (symbolic) execution
+def imem_p1 :=
+  #[
+  addi t0 t0 0x20,   --00
+  ]
+
+-- prove that the pc is 0x04 after executing one clock cycle
+theorem prog1 : ∀ (rf : Regfile) (dm: DMem),
+    let (_rf', _dm', pc') := eval imem_p1 1 0x00 rf dm
+    pc' = 0x04
+  := by
+    simp [eval, imem_p1, instr_eval, instr]
+
+-- prove that reg t0 has increased by 0x20 (independent on initial value)
+-- notice the value might have overflowed (we have wrapping arithmetics)
+theorem prog1b : ∀ (rf : Regfile) (dm: DMem),
+    let (rf', _dm', _pc') := eval imem_p1 1 0x00 rf dm
+    rf'[t0.toNat] = (rf[t0.toNat] + 0x20)
+  := by
+    simp [eval, imem_p1, instr_eval, instr, Regfile.w, Regfile.r, t0, zero]
+
+-- a bit more complex, here we first update t1 and based on that t2
+def imem_p2 :=
+  #[
+  addi t1 t0 0x20,   --00
+  addi t2 t1 0x20,   --04
+  ]
+
+-- prove the value of t1 after 2 clock cycles
+theorem prog2 : ∀ (rf : Regfile) (dm: DMem),
+    let (rf', _dm', _pc') := eval imem_p2 2 0x00 rf dm
+    rf'[t1.toNat] = (rf[t0.toNat] + 0x20)
+  := by
+    simp [eval, imem_p2, instr_eval, instr, Regfile.w, Regfile.r, t0, t1, t2, zero]
+
+-- prove the value of t2 after 2 clock cycles
+-- this should now be initial t0 + 0x40
+theorem prog2b : ∀ (rf : Regfile) (dm: DMem),
+    let (rf', _dm', _pc') := eval imem_p2 2 0x00 rf dm
+    rf'[t2.toNat] = (rf[t0.toNat] + 0x40)
+  := by
+    simp [eval, imem_p2, instr_eval, instr, Regfile.w, Regfile.r, t0, t1, t2, zero]
+    bv_decide
+
+-- now lets try to prove the implementation of arithmetic summation
+
+-- specification arithmetic sum
+def sum (n:Nat) : Nat :=
+  match n with
+  | 0     => 0
+  | n + 1 => n + 1 + (sum n)
+
+#eval (sum 3) -- 3 + 2 + 1 = 6
+
+-- implementation arithmetic sum
+-- let n = 3; // sum = 1 + 2 + 3 = 6
+-- let mut sum = 0;
+-- for i in 1..=n {
+--  sum += i;
+-- }
+
+-- assembly version
+-- m :   t0 (n + 1)
+-- sum : t1
+-- i :   t2
+def imem_sum :=
+  #[
+  addi t0   zero 0x4  ,--00 m = n + 1
+  addi t1   zero 0x0  ,--04 sum = 0
+  addi t2   zero 0x0  ,--08 i = 0
+  slt  at'  t2   t0   ,--0c i < m
+  beq  at'  zero 3    ,--10 for: !(i < m) -> end
+  add  t1   t1   t2   ,--14   sum = sum + i
+  addi t2   t2   1    ,--18   i = i + 1
+  j    3              ,--1c   j for:
+  beq  zero zero (-1) ,--20 end: b end
+  ]
+
+#eval (eval imem_sum 25 0x00 rf dm).fst[t1.toNat]
+
+theorem prog_sum : ∀ (rf : Regfile) (dm: DMem),
+    let (rf', _dm', _pc') := eval imem_sum 25 0x00 rf dm
+    rf'[t1.toNat] = 6
+  := by
+    simp [eval, imem_sum, instr_eval, instr, Regfile.w, Regfile.r, at', t0, t1, t2, zero]
+
+-- We want to prove that for all n, the program computes the sum according to the specification
+-- However we have to assume:
+--   sum n = (sum n: Bv32), that is the result fits 32 bits
+--   pc = 0x20, the program has run to end
+theorem prog_sum_proof : ∀ (rf : Regfile) (dm: DMem) (n f: Nat),
+    let (rf', dm', pc') := eval imem_sum f 0x00 rf dm
+    sum n = (sum n: Bv32) -> (pc' = 0x20) -> (rf'[t1.toNat] = sum n)
+  := by
+    simp [eval, imem_sum, instr_eval, instr, Regfile.w, Regfile.r, at', t0, t1, t2, zero]
+    sorry
